printer.mli
@@ -211,3 +211,9 @@ val print_string_lit : string -> string
 val hex_digits : nat -> z -> string -> string
 
 val print_hex : z -> string
+
+type goExpr =
+| GERaw of string
+| GEBin of nat * string * goExpr * goExpr
+
+val print_prec : nat -> goExpr -> string
